\classheader{2018-11-07}

\begin{lemma}
	In this case $\bX$ is independent of $(X_1 - \bX, X_1 - \bX, \ldots, X_n - \bX)$
\end{lemma}
\begin{lemma}
	IF $X_i$s are i.i.d $\mathcal{N}(\mu, \sigma^2)$ then $\bX$ and $s^2$ are independent (follows immediately from earlier lemma).
\end{lemma}
\begin{lemma}
	If $X_i \sim $ i.i.d $\mathcal{N}(\mu, \sigma^2)$ then $\frac{(n-1)s^2}{\sigma^2} \sim \chi^2 \quad (n-1 \text{ degrees of freedom})$
\end{lemma}
So if $X_i, \ldots, X_n \sim$ i.i.d. $\mathcal{N}(\mu, \sigma^2)$
\begin{gather*}
	\text{We  know} \quad	\frac{\bX - \mu}{\sigma / \sqrt{n}} \sim \mathcal{N}(0,1)\\
	\text{We also know} \quad \frac{s^2 (n-1)}{\sigma^2} \sim \chi^2 (n-1 \quad df)\\
	\frac{s^2 (n-1)}{\sigma^2} \quad \text{is independent of} \quad \frac{\bX - \mu}{\sigma / \sqrt{n}}
\end{gather*}
So we find
\begin{gather*}
	\frac{\frac{\bX - \mu}{\sigma / \sqrt{n}}}{\sqrt{\frac{s^2 (n-1)}{\sigma^2}}} \sim t(n-1 \quad df)\\
	= \frac{\frac{\bX - \mu}{\sigma / \sqrt{n}}}{s / \sigma} = \boxed{\frac{\bX - \mu}{s / \sqrt{n}} \sim t(n-1 \quad df) }
\end{gather*}
So we want to understand hypotheses about $\mu$ e.g.
\begin{center}
	$H_0: \mu = \mu_0$, \quad $\sigma^2$ unknown (composite null)\\
	vs $H_1: \mu \neq \mu_0$, \quad $\sigma^2$ unknown (composite altetrnate)\\
\end{center}
But to build a framework for testing such hypotheses, we will consider \underline{generalized likelihood ratio test}. Suppose we would like to test:
\begin{gather*}
	H_0: \theta \in \Theta_0\\
		H_a: \theta \in \Theta_a\\
		\text{Suppose} \quad \Theta = \Theta_0 \bigcup \Theta_a
\end{gather*}
Consider $l$ = likelihood: $l(X_1, \ldots, X_n | \theta)$. Define:
\begin{gather*}
	\Lambda^* = \frac{\max\limits_{\theta \in \Theta_0} l(X_1, \ldots, X_n | \theta) }{\max\limits_{\theta \in \Theta} l(X_1, \ldots, X_n | \theta) }
\end{gather*}
$\Lambda^*$ is called the generalized ratio and the test procedure in which we reject $H_0$ if $\Lambda^* \leq c$ is called GLRT or \underline{generalized likelihood ratio test}. \\\\
In out class, $\Theta_0$, and $\Theta_a$ will generally be "nice" subsets of Euclidean space, whose dimension is well defined and straight forward to calculate.
\begin{example-N}
	\begin{gather*}
		\Theta = \{ (\mu, \sigma^2) : \mu \in \mathbb{R}, \sigma^2 > 0 \}\\
		\dim \Theta = 2, \text{ if } \Theta_0 = \{ \theta : \mu = \mu_0, \sigma^2 = \sigma_0^2  \} \\
		\text{Note} \quad \dim \Theta_0 = 0
	\end{gather*}
\end{example-N}
Suppose we consider $\mu > \mu_0$, $\sigma^2 = \sigma^2_0$
\begin{gather*}
	\text{Then if} \quad \Theta_0 = \{ \theta: \mu > \mu_0, \sigma^2 = \sigma^2_0 \}, \quad \dim \Theta_0 = 1\\
	\text{If} \quad \Theta_0 = \{ \theta: \mu > \mu_0, \sigma^2 > \sigma^2_0 \}, \quad \dim \Theta_0 = 2\\
\end{gather*}
\begin{theorem}
	Under Certain regularity conditions, $-2 \log \Lambda^*$ has $n \rightarrow \infty$, an asymptotic distribution given by $\chi^2$ $(\dim \Theta - \dim \Theta_0)$
\end{theorem}
\begin{example-N}
	Let $X_1, \ldots, X_n \sim$ i.i.d. $\mathcal{N}(\mu, \sigma^2)$. Consider
	\begin{gather*}
		H_0: \mu = \mu_0\\
		H_a: \mu \leq \mu_0
	\end{gather*}
	Suppose $\sigma^2$ is known (all this happens when null is true)
	\begin{gather*}
		\Theta = \{ \mu \in \mathbb{R} \}, \quad \dim \Theta = 1 \text{ and } \dim \Theta_0 = 0\\
		\Lambda^* = \frac{\max\limits_{\theta \in \Theta_0} l(X_1, \ldots, X_n | \theta) }{\max\limits_{\theta \in \Theta} l(X_1, \ldots, X_n | \theta) }\\
		\Lambda^* = \frac{f(x_1, \ldots, x_n | \mu_0, \sigma^2)}{\max\limits_{\mu} f(x_1, \ldots, x_n | \mu_0, \sigma^2)}\\
		\vdots\\
		\log \Lambda^* = \frac{-1}{2\sigma^2} \sum (X_i - \mu_0)^2 + \frac{1}{2\sigma^2} \sum (X_i - \bX)^2\\
		\vdots\\
		= \frac{2\mu_0}{2\sigma^2} n \bX - \frac{n\mu_0^2}{2\sigma^2} - \frac{n\bX^2}{2\sigma^2}\\ = \frac{-n}{2\sigma^2} (\bX^2 - 2\mu \bX + \mu_0^2)\\
		= \frac{-n}{2\sigma^2} (\bX - \mu_0)^2\\
		\frac{-1}{2} \underbrace{\bigg(\frac{\bX - \mu_0}{\sigma / \sqrt{n}} \bigg)^2}_{\sim \mathcal{N}(0, 1) \textbf{ under $H_0$}}
	\end{gather*}
	Hence Wilks theorem 
	\begin{gather*}
		-2 \log \Lambda^* = \bigg(\frac{\bX - \mu_0}{\sigma / \sqrt{n}} \bigg)^2 \sim \chi^2_{1 df}
	\end{gather*}
\end{example-N}
\underline{Wilks} under regularity conditions $-2 \log \Lambda^*$ converges in distribution under $H_0$ to $\chi^2(\dim \Theta - \dim \Theta_0)$